RocqOfRust/revm/revm_interpreter/instructions/simulate/system/gas.v
@@ -5,8 +5,10 @@ Require Import revm.revm_interpreter.instructions.simulate.macros.
 Require Import revm.revm_interpreter.links.gas.
 Require Import revm.revm_interpreter.links.interpreter.
 Require Import revm.revm_interpreter.links.interpreter_types.
+Require Import revm.revm_interpreter.simulate.gas.
 Require Import revm.revm_interpreter.simulate.interpreter_types.
 Require Import ruint.links.lib.
+Require Import ruint.simulate.from.
 
 Definition gas
     {WIRE : Set} `{Link WIRE}
@@ -19,7 +21,7 @@ Definition gas
     IInterpreterTypes.(InterpreterTypes.LoopControl_for_Control).(LoopControl.gas)
       .(RefStub.projection) interpreter.(Interpreter.control) in
   push_macro interpreter
-    {| Uint.value := i[gas.(Gas.remaining)] |}
+    (Impl_Uint.from gas.(Gas.remaining))
     id
     (fun interpreter => interpreter)
   ).
@@ -28,18 +30,35 @@ Lemma gas_eq
     {WIRE H : Set} `{Link WIRE} `{Link H}
     {WIRE_types : InterpreterTypes.Types.t} `{InterpreterTypes.Types.AreLinks WIRE_types}
     (run_InterpreterTypes_for_WIRE : InterpreterTypes.Run WIRE WIRE_types)
+    (IInterpreterTypes : InterpreterTypes.C WIRE_types)
+    (InterpreterTypesEq :
+      InterpreterTypes.Eq.t WIRE WIRE_types run_InterpreterTypes_for_WIRE IInterpreterTypes)
     (interpreter : Interpreter.t WIRE WIRE_types)
     (host : H) :
   let ref_interpreter := make_ref 0 in
   let ref_host := make_ref (A := H) 1 in
-  exists stack' : Stack.t,
-    {{
-      SimulateM.eval_f
-        (run_gas run_InterpreterTypes_for_WIRE ref_interpreter ref_host)
-        [interpreter; host]%stack 🌲
-      (
-        Output.Success tt,
-        stack'
-      )
-    }}.
-Admitted.
+  {{
+    SimulateM.eval_f
+      (run_gas run_InterpreterTypes_for_WIRE ref_interpreter ref_host)
+      ([interpreter; host]%stack) 🌲
+    (
+      Output.Success tt,
+      [gas interpreter; host]%stack
+    )
+  }}.
+Proof.
+  intros.
+  with_strategy transparent [run_gas] unfold gas, run_gas; cbn.
+  gas_macro_eq InterpreterTypesEq.
+  s. {
+    apply InterpreterTypesEq.
+  }
+  s. {
+    apply Impl_Gas.remaining_eq.
+  }
+  s. {
+    s_apply Impl_Uint.from_eq.
+  }
+  push_macro_eq InterpreterTypesEq.
+  s.
+Qed.
