RocqOfRust/revm/revm_interpreter/instructions/simulate/memory/mload.v
@@ -5,6 +5,7 @@ Require Import core.ops.simulate.deref.
 Require Import core.simulate.option.
 Require Import revm.revm_context_interface.links.host.
 Require Import revm.revm_interpreter.gas.simulate.constants.
+Require Import revm.revm_interpreter.instructions.links.memory.mload.
 Require Import revm.revm_interpreter.instructions.simulate.macros.
 Require Import revm.revm_interpreter.interpreter.simulate.shared_memory.
 Require Import revm.revm_interpreter.links.gas.
@@ -18,31 +19,41 @@ Require Import ruint.links.lib.
 Require Import ruint.simulate.bytes.
 Require Import ruint.simulate.from.
 
-Require Import revm.revm_interpreter.instructions.links.memory.mload.
-
 Definition mload
     {WIRE : Set} `{Link WIRE}
     {WIRE_types : InterpreterTypes.Types.t} `{InterpreterTypes.Types.AreLinks WIRE_types}
-    `{!InterpreterTypes.C WIRE_types}
+    `{IInterpreterTypes : !InterpreterTypes.C WIRE_types}
     (interpreter : Interpreter.t WIRE WIRE_types) :
     Interpreter.t WIRE WIRE_types :=
   gas_macro interpreter constants.VERYLOW id (fun interpreter =>
-  popn_top_macro interpreter 0 id (fun _ top interpreter =>
-  let top := top.(RefStub.projection) interpreter.(Interpreter.stack) in
+  popn_top_macro interpreter 0 id (fun _ top_stub interpreter =>
+  let top := top_stub.(RefStub.projection) interpreter.(Interpreter.stack) in
   as_usize_or_fail_macro interpreter top None id (fun offset interpreter =>
   resize_memory_macro interpreter offset 32 id (fun interpreter =>
-      (* let IInterpreterTypes := _ in
-      let memory_synthetic :=
-        IInterpreterTypes.(InterpreterTypes.MemoryTrait_for_Memory).(MemoryTrait.slice_len)
-          interpreter.(Interpreter.memory) offset 32 in
-      let deref_stub :=
-        IInterpreterTypes.(InterpreterTypes.MemoryTrait_for_Memory).(MemoryTrait.Deref_for_Synthetic1).(Deref.deref) in
-      let bytes := deref_stub.(RefStub.projection) memory_synthetic in
-      let value := u256_from_be_bytes bytes in
-      let stack := top.(RefStub.injection) interpreter.(Interpreter.stack) value in
-      interpreter <| Interpreter.stack := stack |> *)
-    interpreter
-    )))).
+  let memory_slice :=
+    IInterpreterTypes.(InterpreterTypes.MemoryTrait_for_Memory).(MemoryTrait.slice_len)
+      interpreter.(Interpreter.memory) offset 32 in
+  let deref_stub :=
+    IInterpreterTypes.(InterpreterTypes.MemoryTrait_for_Memory).(MemoryTrait.Deref_for_Synthetic1).(Deref.deref) in
+  let bytes := deref_stub.(RefStub.projection) memory_slice in
+  (* [Impl_Uint.try_from_be_slice_eq] in the success case *)
+  let value := {| Uint.value := Impl_Uint.bytes_to_value bytes |} in
+  let stack := top_stub.(RefStub.injection) interpreter.(Interpreter.stack) value in
+  interpreter <| Interpreter.stack := stack |>
+  )))).
+
+Lemma good_size
+    {WIRE_types : InterpreterTypes.Types.t} `{InterpreterTypes.Types.AreLinks WIRE_types}
+    `{IInterpreterTypes : !InterpreterTypes.C WIRE_types}
+    mem
+    (offset : usize) :
+  List.length
+    (IInterpreterTypes.(InterpreterTypes.MemoryTrait_for_Memory).(MemoryTrait.Deref_for_Synthetic1)
+    .(Deref.deref).(RefStub.projection)
+    (IInterpreterTypes.(InterpreterTypes.MemoryTrait_for_Memory).(MemoryTrait.slice_len) mem
+      offset 32)) =
+  32%nat.
+Admitted.
 
 Lemma mload_eq
     {WIRE H : Set} `{Link WIRE} `{Link H}
@@ -86,7 +97,13 @@ Proof.
   }
   s. {
     apply Impl_Option.unwrap_eq.
-    admit.
+    set (mem := snd _).
+    set (slice := _.(MemoryTrait.Deref_for_Synthetic1).(Deref.deref).(RefStub.projection) _).
+    assert (H_size : List.length slice = 32%nat) by apply good_size.
+    unfold Impl_Uint.try_from_be_slice.
+    rewrite H_size; cbn.
+    reflexivity.
   }
   s.
-Admitted.
+  now destruct _.(MemoryTrait.resize).
+Qed.
