RocqOfRust/revm/revm_interpreter/instructions/simulate/memory/msize.v
@@ -5,6 +5,7 @@ Require Import core.ops.simulate.deref.
 Require Import core.simulate.option.
 Require Import revm.revm_context_interface.links.host.
 Require Import revm.revm_interpreter.gas.simulate.constants.
+Require Import revm.revm_interpreter.instructions.links.memory.msize.
 Require Import revm.revm_interpreter.instructions.simulate.macros.
 Require Import revm.revm_interpreter.interpreter.simulate.shared_memory.
 Require Import revm.revm_interpreter.links.gas.
@@ -18,21 +19,18 @@ Require Import ruint.links.lib.
 Require Import ruint.simulate.bytes.
 Require Import ruint.simulate.from.
 
-Require Import revm.revm_interpreter.instructions.links.memory.msize.
-
 Definition msize
     {WIRE : Set} `{Link WIRE}
     {WIRE_types : InterpreterTypes.Types.t} `{InterpreterTypes.Types.AreLinks WIRE_types}
-    `{!InterpreterTypes.C WIRE_types}
+    `{IInterpreterTypes : !InterpreterTypes.C WIRE_types}
     (interpreter : Interpreter.t WIRE WIRE_types) :
     Interpreter.t WIRE WIRE_types :=
   gas_macro interpreter constants.BASE id (fun interpreter =>
-    let IInterpreterTypes := _ in
-    let size :=
-      IInterpreterTypes.(InterpreterTypes.MemoryTrait_for_Memory).(MemoryTrait.size)
-        interpreter.(Interpreter.memory) in
-    let value : aliases.U256.t := {| Uint.value := i[size] |} in
-    push_macro interpreter value id (fun interpreter => interpreter)).
+  let size :=
+    IInterpreterTypes.(InterpreterTypes.MemoryTrait_for_Memory).(MemoryTrait.size)
+      interpreter.(Interpreter.memory) in
+  let value : aliases.U256.t := Impl_Uint.from size in
+  push_macro interpreter value id (fun interpreter => interpreter)).
 
 Lemma msize_eq
     {WIRE H : Set} `{Link WIRE} `{Link H}
