RocqOfRust/revm/revm_interpreter/instructions/simulate/system/address.v
@@ -1,4 +1,7 @@
 Require Import simulate.RocqOfRust.
+Require Import alloy_primitives.bits.simulate.address.
+Require Import alloy_primitives.bits.simulate.fixed.
+Require Import core.convert.simulate.mod.
 Require Import revm.revm_interpreter.gas.simulate.constants.
 Require Import revm.revm_interpreter.instructions.links.system.address.
 Require Import revm.revm_interpreter.instructions.simulate.macros.
@@ -6,6 +9,7 @@ Require Import revm.revm_interpreter.instructions.simulate.utility.
 Require Import revm.revm_interpreter.links.interpreter.
 Require Import revm.revm_interpreter.links.interpreter_types.
 Require Import revm.revm_interpreter.simulate.interpreter_types.
+Require Import ruint.links.from.
 
 Definition address
     {WIRE : Set} `{Link WIRE}
@@ -27,18 +31,35 @@ Lemma address_eq
     {WIRE H : Set} `{Link WIRE} `{Link H}
     {WIRE_types : InterpreterTypes.Types.t} `{InterpreterTypes.Types.AreLinks WIRE_types}
     (run_InterpreterTypes_for_WIRE : InterpreterTypes.Run WIRE WIRE_types)
+    (IInterpreterTypes : InterpreterTypes.C WIRE_types)
+    (InterpreterTypesEq :
+      InterpreterTypes.Eq.t WIRE WIRE_types run_InterpreterTypes_for_WIRE IInterpreterTypes)
     (interpreter : Interpreter.t WIRE WIRE_types)
     (host : H) :
   let ref_interpreter := make_ref 0 in
   let ref_host := make_ref (A := H) 1 in
-  exists stack' : Stack.t,
     {{
       SimulateM.eval_f
         (run_address run_InterpreterTypes_for_WIRE ref_interpreter ref_host)
         [interpreter; host]%stack 🌲
       (
         Output.Success tt,
-        stack'
+        [address interpreter; host]%stack
       )
     }}.
-Admitted.
+Proof.
+  intros.
+  with_strategy transparent [run_address] unfold address, run_address; cbn.
+  gas_macro_eq InterpreterTypesEq.
+  s. {
+    apply InterpreterTypesEq.
+  }
+  s. {
+    s_apply Impl_Address.into_word_eq.
+  }
+  s. {
+    apply Impl_Into_for_From_T.Eq.I.
+  }
+  push_macro_eq InterpreterTypesEq.
+  s.
+Qed.
